arm_hyp proof: update for explicit fpu changes
Signed-off-by: Corey Lewis <corey.lewis@proofcraft.systems>

proof/invariant-abstract/ARM_HYP/ArchInvariants_AI.thy
@@ -743,6 +743,14 @@ where
 |  _ \<Rightarrow> False"
 
 
+(* arch_tcb_live stub; there is no state in the arch specific part of TCBs on this platform that
+   marks a TCB as live *)
+definition arch_tcb_live :: "arch_tcb \<Rightarrow> bool" where
+  "arch_tcb_live arch_tcb \<equiv> False"
+
+definition valid_cur_fpu :: "'z::state_ext state \<Rightarrow> bool" where
+  "valid_cur_fpu \<equiv> \<top>"
+
 definition
   is_vcpu :: "kernel_object \<Rightarrow> bool"
 where
@@ -1260,7 +1268,6 @@ lemma valid_pd_kernel_mappings [iff]:
       = valid_pd_kernel_mappings uses s"
   by (rule ext, simp add: valid_pd_kernel_mappings_def)
 
-
 (* FIXME: Clagged *)
 lemma get_cap_update [iff]:
   "(fst (get_cap p (f s)) = {(cap, f s)}) = (fst (get_cap p s) = {(cap, s)})"
@@ -1331,6 +1338,10 @@ lemma valid_vspace_objs_update' [iff]:
   "valid_vspace_objs (f s) = valid_vspace_objs s"
   by (simp add: valid_vspace_objs_def)
 
+lemma valid_cur_fpu_update [iff]:
+  "valid_cur_fpu (f s) = valid_cur_fpu s"
+  by (auto simp: valid_cur_fpu_def)
+
 end
 
 context Arch begin arch_global_naming
@@ -1364,6 +1375,10 @@ lemma valid_arch_state_lift:
    apply (case_tac "arm_current_vcpu x"; simp add: split_def)
     apply (wp arch vcpus typs hoare_vcg_conj_lift hoare_vcg_const_Ball_lift)+
   done
+
+lemma valid_cur_fpu_updates[simp]:
+  "\<And>f. valid_cur_fpu (arch_state_update f s) = valid_cur_fpu s"
+  by (auto simp: valid_cur_fpu_def)
 
 lemma aobj_at_default_arch_cap_valid:
   assumes "ty \<noteq> ASIDPoolObj"
@@ -2107,9 +2122,9 @@ lemma aa_type_vcpuD:
   by (clarsimp simp: aa_type_def
                split: arch_kernel_obj.splits if_split_asm)
 
-lemma global_refs_asid_table_update [iff]:
-  "global_refs (s\<lparr>arch_state := arm_asid_table_update f (arch_state s)\<rparr>) = global_refs s"
-  by (simp add: global_refs_def)
+lemma global_refs_updates[simp]:
+  "\<And>f. global_refs (s\<lparr>arch_state := arm_asid_table_update f (arch_state s)\<rparr>) = global_refs s"
+  by (auto simp: global_refs_def)
 
 lemma pspace_in_kernel_window_arch_update[simp]:
   "arm_kernel_vspace (f (arch_state s)) = arm_kernel_vspace (arch_state s)
@@ -2403,21 +2418,19 @@ lemma valid_tcb_arch_ref_lift:
   "tcb_arch_ref t = tcb_arch_ref t' \<Longrightarrow> valid_arch_tcb (tcb_arch t) = valid_arch_tcb (tcb_arch t')"
   by (simp add: valid_arch_tcb_def tcb_arch_ref_def)
 
-lemma valid_arch_tcb_context_update[simp]:
-  "valid_arch_tcb (tcb_context_update f t) = valid_arch_tcb t"
-  unfolding valid_arch_tcb_def obj_at_def by simp
+lemma valid_arch_tcb_simps[simp]:
+  "\<And>f. valid_arch_tcb (tcb_context_update f t) = valid_arch_tcb t"
+  by (simp add: valid_arch_tcb_def)+
 
-lemma valid_arch_arch_tcb_context_set[simp]:
-  "valid_arch_tcb (arch_tcb_context_set a t) = valid_arch_tcb t"
-  by (simp add: arch_tcb_context_set_def)
-
-lemma valid_arch_arch_tcb_set_registers[simp]:
-  "valid_arch_tcb (arch_tcb_set_registers a t) = valid_arch_tcb t"
-   by (simp add: arch_tcb_set_registers_def)
+lemma valid_arch_tcb_context_simps[simp]:
+  "\<And>a. valid_arch_tcb (arch_tcb_context_set a t) = valid_arch_tcb t"
+  "\<And>a. valid_arch_tcb (arch_tcb_set_registers a t) = valid_arch_tcb t"
+  by (simp add: arch_tcb_context_set_def arch_tcb_set_registers_def)+
 
 lemma tcb_arch_ref_simps[simp]:
   "\<And>f. tcb_arch_ref (tcb_ipc_buffer_update f tcb) = tcb_arch_ref tcb"
   "\<And>f. tcb_arch_ref (tcb_mcpriority_update f tcb) = tcb_arch_ref tcb"
+  "\<And>f. tcb_arch_ref (tcb_flags_update f tcb) = tcb_arch_ref tcb"
   "\<And>f. tcb_arch_ref (tcb_ctable_update f tcb) = tcb_arch_ref tcb"
   "\<And>f. tcb_arch_ref (tcb_vtable_update f tcb) = tcb_arch_ref tcb"
   "\<And>f. tcb_arch_ref (tcb_reply_update f tcb) = tcb_arch_ref tcb"
@@ -2453,6 +2466,16 @@ lemma hyp_live_tcb_simps[simp]:
   "\<And>f. hyp_live (TCB (tcb_priority_update f tcb)) = hyp_live (TCB tcb)"
   "\<And>f. hyp_live (TCB (tcb_time_slice_update f tcb)) = hyp_live (TCB tcb)"
   by (simp_all add: hyp_live_tcb_def)
+
+lemma arch_tcb_live_simps[simp]:
+  "\<And>f. arch_tcb_live (tcb_context_update f arch_tcb) = arch_tcb_live arch_tcb"
+  "\<And>f. arch_tcb_live (tcb_vcpu_update f arch_tcb) = arch_tcb_live arch_tcb"
+  by (simp_all add: arch_tcb_live_def)
+
+lemma arch_tcb_live_context_simps[simp]:
+  "\<And>f. arch_tcb_live (arch_tcb_context_set f arch_tcb) = arch_tcb_live arch_tcb"
+  "\<And>f. arch_tcb_live (arch_tcb_set_registers f arch_tcb) = arch_tcb_live arch_tcb"
+  by (simp_all add: arch_tcb_context_set_def arch_tcb_set_registers_def)
 
 
 lemma valid_arch_tcb_pspaceI:
